src/tools/lifter/bir_inst_liftingScript.sml
@@ -4,6 +4,7 @@ open bir_expTheory HolBACoreSimps;
 open bir_typing_expTheory bir_valuesTheory
 open bir_envTheory bir_immTheory bir_imm_expTheory
 open bir_immSyntax bir_programTheory wordsTheory
+open bir_auxiliaryTheory
 open bir_mem_expTheory bir_bool_expTheory
 open bir_program_env_orderTheory
 open bir_program_blocksTheory
@@ -13,11 +14,13 @@ open bir_lifting_machinesTheory
 open bir_interval_expTheory
 open bir_update_blockTheory
 open bir_lifting_machinesLib
+open pred_setTheory
 
 (* This theory defines what it means for a block and a whole program
    to be corresponding to a machine instruction *)
 
 val _ = new_theory "bir_inst_lifting";
+
 
 
 (*****************************)
@@ -87,7 +90,7 @@ val bir_is_lifted_inst_block_def = Define `
 
     (* A condition allowing is to get extra information into our reasoning. It can
        say for example which of the theorems of produced by the step theorem we are
-       dealing with and just assume at the meta leval some of it's preconditions
+       dealing with and just assume at the meta level some of it's preconditions
        instead of asserting them in BIR. This allows to discard them later by looking
        at the control flow of a larger bir program containing the block. *)
     (ms_case_cond : 'ms -> bool)
@@ -146,10 +149,71 @@ val bir_is_lifted_inst_block_def = Define `
            (bmr_rel r bs' ms')))`;
 
 
-(**************************)
-(* Computing such a block *)
-(**************************)
 
+
+(**********************************************)
+(* Deriving bir_is_lifted_inst_block theorems *)
+(**********************************************)
+
+(* The main functionality of the instruction lifter to lift single machine instructions
+   and as justification provide bir_is_lifted_inst_block theorems. These are
+   later combined to have a connection for whole programs instead of single blocks,
+   but this is comparably simple and non-machine dependent.
+
+   So, given some step-theorem describing the behaviour of our machine, that
+   describes the behaviour of one step of a machine usually using the assumptions that
+
+   - some instr is stored at the PC pointer in memory
+   - PC has a certain value
+   - some extra conditions hold
+
+   and further given
+
+   - a machine description "r"
+   - a condition "ms_case_cond" we may assume from the calling context
+   - a region of memory we should not touch "mu"
+
+   we want to derive
+
+   - a memory mapping "mm" that describes the instruction stored in mem
+   - a label "l" corresponding to the PC
+   - and most importantly a bir-block "bl" such that
+
+   bir_is_lifted_inst_block r ms_case_cond l mu mm bl
+
+   holds.
+
+   To do this, we want to do as little real work as possible at runtime.
+   So preproved theorems about assert-update-blocks and the record r are
+   used. The theorem "bir_is_lifted_inst_block_COMPUTE" captures at a high
+   level of abstraction how to do such a computation.
+
+   However, "bir_is_lifted_inst_block_COMPUTE" is not how one would really
+   like to reason automatically. It is at a high, intuitive level of abstraction.
+   Many properties esp. things like
+
+   - variable names being well-formed
+   - var names being distinct
+   - vars are declared properly
+   ...
+
+   are demanded by the preconditions of "bir_is_lifted_inst_block_COMPUTE"
+   explicitly, while they could be derived by e.g. well-formedness properties
+   of the machine lifting record "r". So, there is an
+   optimised version "bir_is_lifted_inst_block_COMPUTE_OPTIMISED".
+   The idea is the same as for ""bir_is_lifted_inst_block_COMPUTE". However,
+   not the preconditions are streamlined for efficient instantiation in the
+   automation provided by bir_inst_liftingLib.
+
+   Both for "bir_is_lifted_inst_block_COMPUTE" and
+   "bir_is_lifted_inst_block_COMPUTE_OPTIMISED" many auxiliary definitions are
+   introduced.
+*)
+
+
+(*-----------------------*)
+(* Auxiliary definitions *)
+(*-----------------------*)
 
 val bir_is_lifted_inst_block_COMPUTE_ms'_COND_def = Define
   `bir_is_lifted_inst_block_COMPUTE_ms'_COND r ms al_step ms' <=>
@@ -157,7 +221,7 @@ val bir_is_lifted_inst_block_COMPUTE_ms'_COND_def = Define
      ((EVERY (\a. bir_assert_desc_value a) al_step) ==>
       (r.bmr_step_fun ms = SOME ms')) /\
 
-     (* This machine step statisfies the machine state invariants *)
+     (* This machine step satisfies the machine state invariants *)
      ((EVERY (\a. bir_assert_desc_value a) al_step) ==>
       r.bmr_extra ms')`
 
@@ -214,6 +278,11 @@ val bir_is_lifted_inst_block_COMPUTE_eup_COND_def = Define
                | (BMLM v lf) => (bir_var_name var) <> (bir_var_name v)))) /\
      (bir_updateE_SEM eup = BUpdateValE_Jmp (BL_Address (bmr_pc_lf r ms')))`;
 
+
+
+(*-------------*)
+(* The theorem *)
+(*-------------*)
 
 val bir_is_lifted_inst_block_COMPUTE = store_thm ("bir_is_lifted_inst_block_COMPUTE",
 ``!r bl ms_case_cond l mm mu l'.
@@ -373,22 +442,20 @@ ASM_SIMP_TAC std_ss []);
 
 
 
-(***************************)
-(* Finer grained computing *)
-(***************************)
+(**********************************************************)
+(* Efficiently deriving bir_is_lifted_inst_block theorems *)
+(**********************************************************)
 
 (* The lemma bir_is_lifted_inst_block_COMPUTE is worded in such a way that
-   it is comparably easy to show correct. The actual SML code does not need to
-   (and should) not follow it litterally though. There are 2 issues:
+   it is comparably easy to understand for humans. The actual SML code does not need to
+   (and should) not follow it literally though.
 
-   - above certain combinations of invariants / well-formedness conditions are
-     not exploited, since they would lead to more detailed, fidlly proofs.
-     We can exploit them as an optimisation below and thereby safe runtime checks.
+   Please see above for details. *)
 
-   - The computation of UPDATE is weird. We first need to compute
-     imm_ups and mem_up and then use these to compute updates. It is sensible to
-     detangle this in the definitions.
-*)
+
+(*-----------------------*)
+(* Auxiliary definitions *)
+(*-----------------------*)
 
 val bir_is_lifted_inst_block_COMPUTE_ms'_COND_WITH_DESC_OK_def = Define
   `bir_is_lifted_inst_block_COMPUTE_ms'_COND_WITH_DESC_OK r bs ms al_step ms' <=>
@@ -406,7 +473,7 @@ val bir_is_lifted_inst_block_COMPUTE_imm_ups_COND_NO_UPDATES_def = Define
 
      (MAP FST imm_ups = r.bmr_imms) /\
      (!v lf. (MEM (BMLI v lf, NONE) imm_ups) ==>
-             (lf ms' = lf ms)) /\
+                     (lf ms' = lf ms)) /\
 
      (!v lf res. (MEM (BMLI v lf, SOME res) imm_ups) ==>
                  (lf ms' = res))`;
@@ -422,7 +489,98 @@ val bir_is_lifted_inst_block_COMPUTE_imm_ups_COND_UPDATES_def = Define
                  (?up. MEM up updates /\ (bir_updateB_desc_var up = v) /\
                  (bir_updateB_desc_value up = BVal_Imm res)))`
 
-val bir_is_lifted_inst_block_COMPUTE_imm_ups_COND_THM = store_thm ("bir_is_lifted_inst_block_COMPUTE_imm_ups_COND_THM",
+
+val bir_is_lifted_inst_block_COMPUTE_mem_COND_UPDATES_def = Define
+  `bir_is_lifted_inst_block_COMPUTE_mem_COND_UPDATES r bs ms ms' mem_up updates <=>
+     (* Memory update sensible *)
+     (case (mem_up, r.bmr_mem) of
+       | (NONE, BMLM v lf) =>
+             (!up. MEM up updates ==>
+                   (bir_var_name v <> bir_var_name (bir_updateB_desc_var up)))
+       | (SOME res, BMLM v lf) =>
+              (?up.
+              MEM up updates /\ (bir_updateB_desc_var up = v) /\
+              (bir_is_lifted_exp bs.bst_environ (bir_updateB_desc_exp up) (BLV_Mem res))))`;
+
+val bir_is_lifted_inst_block_COMPUTE_mem_COND_NO_UPDATES_def = Define
+  `bir_is_lifted_inst_block_COMPUTE_mem_COND_NO_UPDATES r ms ms' mem_up <=>
+     (case (mem_up, r.bmr_mem) of
+       | (NONE, BMLM v lf) => (
+             (lf ms' = lf ms))
+       | (SOME res, BMLM v lf) =>
+              (lf ms' = res))`;
+
+
+val bir_is_lifted_inst_block_COMPUTE_eup_COND_FIXED_VARS_def = Define
+  `bir_is_lifted_inst_block_COMPUTE_eup_COND_FIXED_VARS r bs eup ms'  <=>
+     bir_updateE_desc_OK bs.bst_environ eup /\
+
+     (case (bir_updateE_desc_var eup) of NONE => T
+       | SOME var => case r.bmr_pc of BMLPC v_pc v_pc_cond _ =>
+         ((var = v_pc) \/ (var = v_pc_cond))) /\
+
+     (bir_updateE_SEM eup = BUpdateValE_Jmp (BL_Address (bmr_pc_lf r ms')))`;
+
+
+val bir_is_lifted_inst_block_COMPUTE_updates_FULL_def = Define
+  `bir_is_lifted_inst_block_COMPUTE_updates_FULL
+      (r: ('a, 'b, 'c) bir_lifting_machine_rec_t) bs
+      (mem_up : ('a word -> 'b word) option)
+      (imm_ups :('c bir_machine_lifted_imm_t # bir_imm_t option) list)
+      (eup :bir_updateE_desc_t) (eup_temp :bool) updates =
+
+     ?updates_imm updates_mem.
+
+     (* imm_ups covered *)
+     ((MAP (\up. (bir_updateB_desc_var up, bir_updateB_desc_value up)) updates_imm) =
+      (MAP (\x. (case x of | (BMLI v _, SOME r) => (v, BVal_Imm r)))
+        (FILTER (\x. IS_SOME (SND x)) imm_ups))) /\
+
+     (* mem_up covered *)
+     (case mem_up of NONE => (updates_mem = []) | SOME res =>
+       (?upd_mem. (updates_mem = [upd_mem]) /\
+           (bir_updateB_desc_var upd_mem = bmr_mem_var r) /\
+           (bir_updateB_desc_value upd_mem =
+             (bir_eval_exp (bir_updateB_desc_exp upd_mem) bs.bst_environ)) /\
+           (bir_is_lifted_exp bs.bst_environ (bir_updateB_desc_exp upd_mem)
+             (BLV_Mem res)))) /\
+
+     (* Nothing else updated *)
+     (PERM updates (updates_imm ++ updates_mem)) /\
+
+     (* imm_ups are lifted properly *)
+     (!var e v use_temp.
+            MEM (BUpdateDescB var e (BVal_Imm v) use_temp) updates_imm ==>
+            bir_is_lifted_imm_exp bs.bst_environ e v) /\
+
+     (* Vars fit *)
+     (!i j var.
+        i < LENGTH updates /\ j < i /\
+        var IN bir_vars_of_exp (bir_updateB_desc_exp (EL i updates)) ==>
+        bir_var_name var <>
+        bir_var_name (bir_updateB_desc_temp_var (EL j updates))) /\
+
+     (!v up v'.
+        eup_temp ==>
+        (bir_updateE_desc_var eup = SOME v) ==>
+        MEM up (updates_imm ++ updates_mem) ==>
+        v' IN  bir_vars_of_exp (bir_updateB_desc_exp up) ==>
+        bir_var_name v <> bir_var_name v') /\
+
+     (!v e up v'.
+        (~eup_temp \/ (bir_updateE_desc_var eup = NONE)) ==>
+        (bir_updateE_desc_exp eup = SOME e) ==>
+        v IN bir_vars_of_exp e ==>
+        MEM up (updates_imm ++ updates_mem) ==>
+        v' IN {bir_updateB_desc_temp_var up; bir_updateB_desc_var up} ==>
+        bir_var_name v <> bir_var_name v')`;
+
+
+(*-----------------------*)
+(* Proving optimised thm *)
+(*-----------------------*)
+
+val bir_is_lifted_inst_block_COMPUTE_imm_ups_COND_THM = prove (
 ``!r ms ms' imm_ups updates. bmr_ok r ==>
    (bir_is_lifted_inst_block_COMPUTE_imm_ups_COND r ms ms' imm_ups updates <=>
     (bir_is_lifted_inst_block_COMPUTE_imm_ups_COND_NO_UPDATES r ms ms' imm_ups /\
@@ -448,30 +606,8 @@ FULL_SIMP_TAC std_ss [bir_machine_lifted_imm_OK_def] >>
 METIS_TAC[bir_is_temp_var_name_REWR]);
 
 
-val bir_is_lifted_inst_block_COMPUTE_mem_COND_UPDATES_def = Define
-  `bir_is_lifted_inst_block_COMPUTE_mem_COND_UPDATES r bs ms ms' mem_up updates <=>
-     (* Memory update sensible *)
-     (case (mem_up, r.bmr_mem) of
-       | (NONE, BMLM v lf) =>
-             (!up. MEM up updates ==>
-                   (bir_var_name v <> bir_var_name (bir_updateB_desc_var up)))
-       | (SOME res, BMLM v lf) =>
-              (?up.
-              MEM up updates /\ (bir_updateB_desc_var up = v) /\
-              (bir_is_lifted_exp bs.bst_environ (bir_updateB_desc_exp up) (BLV_Mem res))))`;
 
-
-
-val bir_is_lifted_inst_block_COMPUTE_mem_COND_NO_UPDATES_def = Define
-  `bir_is_lifted_inst_block_COMPUTE_mem_COND_NO_UPDATES r ms ms' mem_up <=>
-     (case (mem_up, r.bmr_mem) of
-       | (NONE, BMLM v lf) => (
-             (lf ms' = lf ms))
-       | (SOME res, BMLM v lf) =>
-              (lf ms' = res))`;
-
-
-val bir_is_lifted_inst_block_COMPUTE_mem_COND_THM = store_thm ("bir_is_lifted_inst_block_COMPUTE_mem_COND_THM",
+val bir_is_lifted_inst_block_COMPUTE_mem_COND_THM = prove (
 ``!r bs ms ms' mem_up updates. bmr_ok r ==>
    (bir_is_lifted_inst_block_COMPUTE_mem_COND r bs ms ms' mem_up updates <=>
     (bir_is_lifted_inst_block_COMPUTE_mem_COND_NO_UPDATES r ms ms' mem_up /\
@@ -495,39 +631,21 @@ REV_FULL_SIMP_TAC std_ss [bmr_ok_def, bir_machine_lifted_mem_OK_def] >>
 METIS_TAC[bir_is_temp_var_name_REWR]);
 
 
+val bir_is_lifted_inst_block_COMPUTE_eup_COND_remove_var = prove (
+``!r eup eup_temp ms'.
+bir_is_lifted_inst_block_COMPUTE_eup_COND r eup ms' ==>
+bir_is_lifted_inst_block_COMPUTE_eup_COND r
+  (if eup_temp then eup else bir_updateE_desc_remove_var eup) ms'``,
 
-val bir_is_lifted_inst_block_COMPUTE_al_mem_COND_WITH_DESC_OK_INTRO_NONE = store_thm (
-  "bir_is_lifted_inst_block_COMPUTE_al_mem_COND_WITH_DESC_OK_INTRO_NONE",
-``!r mu bs ms ms'.
-   bir_is_lifted_inst_block_COMPUTE_mem_COND_NO_UPDATES r ms ms' NONE ==>
-   bir_is_lifted_inst_block_COMPUTE_al_mem_COND_WITH_DESC_OK
-            r mu bs ms ms' []``,
-
-SIMP_TAC list_ss [bir_is_lifted_inst_block_COMPUTE_al_mem_COND_WITH_DESC_OK_def,
-  bir_is_lifted_inst_block_COMPUTE_al_mem_COND_def,
-  bir_is_lifted_inst_block_COMPUTE_mem_COND_NO_UPDATES_def,
-  pairTheory.pair_case_thm, bmr_mem_lf_def] >>
-REPEAT STRIP_TAC >>
-Q.EXISTS_TAC `[]` >>
-Cases_on `r.bmr_mem` >>
-FULL_SIMP_TAC (list_ss++bmr_ss) []);
+Cases_on `eup_temp` >> SIMP_TAC std_ss [] >>
+SIMP_TAC (std_ss) [bir_is_lifted_inst_block_COMPUTE_eup_COND_def,
+   bir_updateE_desc_remove_var_REWRS]);
 
 
-val bir_is_lifted_inst_block_COMPUTE_eup_COND_FIXED_VARS_def = Define
-  `bir_is_lifted_inst_block_COMPUTE_eup_COND_FIXED_VARS r eup ms'  <=>
-     (* EUP sensible *)
-     (case (bir_updateE_desc_var eup) of NONE => T
-       | SOME var => case r.bmr_pc of BMLPC v_pc v_pc_cond _ =>
-         ((var = v_pc) \/ (var = v_pc_cond))) /\
-
-     (bir_updateE_SEM eup = BUpdateValE_Jmp (BL_Address (bmr_pc_lf r ms')))`;
-
-
-val bir_is_lifted_inst_block_COMPUTE_eup_COND_FIXED_VARS_THM = store_thm (
-   "bir_is_lifted_inst_block_COMPUTE_eup_COND_FIXED_VARS_THM",
-``!r eup ms'.
+val bir_is_lifted_inst_block_COMPUTE_eup_COND_FIXED_VARS_THM = prove (
+``!r bs eup ms'.
     bmr_ok r ==>
-    bir_is_lifted_inst_block_COMPUTE_eup_COND_FIXED_VARS r eup ms' ==>
+    bir_is_lifted_inst_block_COMPUTE_eup_COND_FIXED_VARS r bs eup ms' ==>
     bir_is_lifted_inst_block_COMPUTE_eup_COND r eup ms'``,
 
 REPEAT GEN_TAC >>
@@ -556,7 +674,271 @@ FULL_SIMP_TAC (std_ss++bmr_ss) [] >>
 FULL_SIMP_TAC (list_ss++bmr_ss) [bmr_vars_def]);
 
 
-val bir_is_lifted_inst_block_COMPUTE_SPLIT = store_thm ("bir_is_lifted_inst_block_COMPUTE_SPLIT",
+
+val bir_is_lifted_inst_block_COMPUTE_updates_FULL_THM = prove (
+``!r bs ms ms' mem_up imm_ups eup eup_temp updates.
+     bmr_ok r ==>
+     bmr_rel r bs ms ==>
+     bir_is_lifted_inst_block_COMPUTE_imm_ups_COND_NO_UPDATES r ms ms' imm_ups ==>
+     bir_is_lifted_inst_block_COMPUTE_eup_COND_FIXED_VARS r bs eup ms' ==>
+
+     bir_is_lifted_inst_block_COMPUTE_updates_FULL r bs mem_up imm_ups eup eup_temp updates ==>
+
+     (bir_is_lifted_inst_block_COMPUTE_mem_COND_UPDATES r bs ms ms' mem_up updates /\
+      bir_is_lifted_inst_block_COMPUTE_imm_ups_COND_UPDATES r ms ms' imm_ups updates /\
+      bir_update_block_desc_OK bs.bst_environ (if eup_temp then eup else bir_updateE_desc_remove_var eup) updates)``,
+
+REPEAT GEN_TAC >> REPEAT DISCH_TAC >>
+FULL_SIMP_TAC std_ss [bir_is_lifted_inst_block_COMPUTE_updates_FULL_def] >>
+`!upd. MEM upd updates_imm ==>
+       (?lf i. (bir_updateB_desc_value upd = BVal_Imm i) /\
+               MEM (BMLI (bir_updateB_desc_var upd) lf, SOME i) imm_ups)` by (
+  REPEAT STRIP_TAC >>
+  `MEM (bir_updateB_desc_var upd, bir_updateB_desc_value upd)
+      (MAP (\up.(bir_updateB_desc_var up,bir_updateB_desc_value up))
+      updates_imm)` by (
+    FULL_SIMP_TAC std_ss [MEM_MAP] >> METIS_TAC[]
+  ) >>
+  POP_ASSUM MP_TAC >>
+  ASM_REWRITE_TAC[] >>
+  SIMP_TAC (list_ss++QI_ss++bmr_ss++DatatypeSimps.expand_type_quants_ss[``:'a bir_machine_lifted_imm_t``])
+    [MEM_MAP, MEM_FILTER, pairTheory.pair_case_thm]
+) >>
+`!upd. MEM upd updates_imm ==>
+       (?lf. MEM (BMLI (bir_updateB_desc_var upd) lf) r.bmr_imms)` by (
+   REPEAT STRIP_TAC >>
+   FULL_SIMP_TAC std_ss [bir_is_lifted_inst_block_COMPUTE_imm_ups_COND_NO_UPDATES_def] >>
+   METIS_TAC[MEM_MAP, pairTheory.FST]
+) >>
+`!up. MEM up updates <=> MEM up (updates_imm ++ updates_mem)` by
+   METIS_TAC[sortingTheory.MEM_PERM] >>
+Cases_on `r.bmr_mem` >> rename1 `BMLM mem_v mem_lf` >>
+
+`MEM mem_v (bmr_vars r)` by (
+  FULL_SIMP_TAC (list_ss++bmr_ss) [bmr_vars_def]
+) >>
+
+`!up.
+  MEM up updates_imm ==>
+  (MEM (bir_updateB_desc_var up) (bmr_vars r) /\
+  (bir_var_name mem_v <> bir_var_name (bir_updateB_desc_var up)))` by (
+
+  REPEAT STRIP_TAC >>
+  Q.PAT_X_ASSUM `bmr_ok r` MP_TAC >>
+  ASM_SIMP_TAC (list_ss++bmr_ss) [bmr_ok_def, bmr_varnames_distinct_def, ALL_DISTINCT_APPEND, bmr_vars_def, MAP_MAP_o, combinTheory.o_DEF] >>
+  REPEAT STRIP_TAC >>
+  `?lf. MEM (BMLI (bir_updateB_desc_var up) lf) r.bmr_imms` by METIS_TAC[] >>
+  SIMP_TAC (std_ss++bmr_ss++DatatypeSimps.expand_type_quants_ss[``:'a bir_machine_lifted_imm_t``]) [
+    MEM_MAP] >>
+  METIS_TAC[]
+) >>
+
+REPEAT STRIP_TAC >- (
+  ASM_SIMP_TAC (std_ss++bmr_ss) [bir_is_lifted_inst_block_COMPUTE_mem_COND_UPDATES_def,
+    pairTheory.pair_case_thm] >>
+  Tactical.REVERSE (Cases_on `mem_up`) >> (
+    FULL_SIMP_TAC (list_ss++bmr_ss) [bmr_mem_var_def]
+  ) >>
+  METIS_TAC[]
+) >- (
+  ASM_SIMP_TAC (std_ss++bmr_ss) [bir_is_lifted_inst_block_COMPUTE_imm_ups_COND_UPDATES_def,
+    pairTheory.pair_case_thm] >>
+
+  Q.PAT_X_ASSUM `bmr_ok r` MP_TAC >>
+  ASM_SIMP_TAC (list_ss++bmr_ss) [bmr_ok_def, bmr_varnames_distinct_def, ALL_DISTINCT_APPEND, bmr_vars_def, MAP_MAP_o, combinTheory.o_DEF] >>
+  `r.bmr_imms = MAP FST imm_ups` by
+    FULL_SIMP_TAC std_ss [bir_is_lifted_inst_block_COMPUTE_imm_ups_COND_NO_UPDATES_def] >>
+  REPEAT STRIP_TAC >- (
+    `?n1. n1 < LENGTH imm_ups /\ (EL n1 imm_ups = (BMLI v lf,NONE))` by METIS_TAC[MEM_EL] >>
+    `?n2 lf' i. n2 < LENGTH imm_ups /\
+                (EL n2 imm_ups = (BMLI (bir_updateB_desc_var up) lf', SOME i))` by
+       METIS_TAC[MEM_EL] >>
+    `n1 <> n2` by (
+      STRIP_TAC >>
+      FULL_SIMP_TAC std_ss []
+    ) >>
+    Q.ABBREV_TAC `vs_imms = (MAP (\i. bir_var_name (case i of BMLI v v2 => v)) r.bmr_imms)` >>
+    `LENGTH vs_imms = LENGTH imm_ups` by (
+       Q.UNABBREV_TAC `vs_imms` >> FULL_SIMP_TAC list_ss []) >>
+    `(EL n1 vs_imms = bir_var_name v) /\
+     (EL n2 vs_imms = bir_var_name v)` by (
+       Q.UNABBREV_TAC `vs_imms` >>
+       FULL_SIMP_TAC (list_ss++bmr_ss) [EL_MAP]
+    ) >>
+    METIS_TAC[EL_ALL_DISTINCT_EL_EQ]
+  ) >- (
+    Cases_on `mem_up` >> REV_FULL_SIMP_TAC list_ss[] >>
+    REV_FULL_SIMP_TAC (list_ss++bmr_ss) [bmr_mem_var_def] >>
+    REPEAT (BasicProvers.VAR_EQ_TAC) >>
+    FULL_SIMP_TAC (list_ss++bmr_ss++QI_ss++DatatypeSimps.expand_type_quants_ss[``:'a bir_machine_lifted_imm_t``]) [MEM_MAP] >>
+    METIS_TAC[]
+  ) >- (
+    `MEM (v, BVal_Imm res) (MAP (\up. (bir_updateB_desc_var up,bir_updateB_desc_value up))
+         updates_imm)` by (
+      ASM_REWRITE_TAC[] >>
+      ASM_SIMP_TAC (list_ss++QI_ss++bir_TYPES_ss++bmr_ss++DatatypeSimps.expand_type_quants_ss[``:'a bir_machine_lifted_imm_t``]) [MEM_MAP, MEM_FILTER, pairTheory.pair_case_thm]
+    ) >>
+    POP_ASSUM MP_TAC >>
+    SIMP_TAC std_ss [MEM_MAP] >>
+    METIS_TAC[]
+  )
+) >>
+
+SIMP_TAC std_ss [bir_update_block_desc_OK_def, bir_update_blockB_desc_OK_def] >>
+
+`bir_updateE_desc_OK bs.bst_environ
+  (if eup_temp then eup else bir_updateE_desc_remove_var eup)` by (
+  FULL_SIMP_TAC (std_ss) [bir_is_lifted_inst_block_COMPUTE_eup_COND_FIXED_VARS_def] >>
+  Cases_on `eup_temp` >> (
+    ASM_SIMP_TAC std_ss [bir_updateE_desc_OK_remove_var]
+  )
+) >>
+
+`EVERY (bir_updateB_desc_OK bs.bst_environ) updates` by (
+  ASM_SIMP_TAC list_ss [EVERY_MEM] >>
+  Cases >> rename1 `BUpdateDescB v e res use_temp` >>
+  STRIP_TAC >- (
+    `?i. res = BVal_Imm i` by METIS_TAC[bir_updateB_desc_value_def] >>
+    `bir_is_lifted_imm_exp bs.bst_environ e i` by METIS_TAC[] >>
+
+    FULL_SIMP_TAC std_ss [bir_updateB_desc_OK_def, bir_is_lifted_imm_exp_def] >>
+    `?lf. MEM (BMLI v lf, SOME i) imm_ups` by METIS_TAC[bir_updateB_desc_value_def,
+       bir_updateB_desc_var_def, bir_val_t_11] >>
+
+    FULL_SIMP_TAC std_ss [bir_is_lifted_inst_block_COMPUTE_imm_ups_COND_NO_UPDATES_def] >>
+    `lf ms' = i` by METIS_TAC[] >>
+    `MEM (BMLI v lf) r.bmr_imms` by  (
+       Q.PAT_X_ASSUM `_ = r.bmr_imms` (ASSUME_TAC o GSYM) >>
+       ASM_SIMP_TAC (std_ss++QI_ss) [MEM_MAP]
+    ) >>
+    `bir_machine_lifted_imm_OK (BMLI v lf)` by METIS_TAC[bmr_ok_def, EVERY_MEM] >>
+    FULL_SIMP_TAC std_ss [bir_machine_lifted_imm_OK_def] >>
+    Q.PAT_X_ASSUM `!ms. _ = bir_var_type _` (MP_TAC o GSYM o Q.SPEC `ms'`) >>
+    ASM_SIMP_TAC std_ss [type_of_bir_val_def] >>
+    `MEM v (bmr_vars r)` by (
+       ASM_SIMP_TAC (list_ss++bmr_ss++DatatypeSimps.expand_type_quants_ss[``:'a bir_machine_lifted_imm_t``]) [bmr_vars_def, MEM_MAP] >>
+       METIS_TAC[]
+    ) >>
+    Cases_on `use_temp` >> (
+      METIS_TAC[EVERY_MEM, bmr_vars_DECLARED, bmr_temp_vars_DECLARED,
+        bmr_vars_IN_TEMP, bir_temp_var_REWRS]
+    )
+  ) >- (
+    Cases_on `mem_up` >> REV_FULL_SIMP_TAC list_ss [] >>
+    REV_FULL_SIMP_TAC list_ss [] >>
+    REPEAT (BasicProvers.VAR_EQ_TAC) >>
+    FULL_SIMP_TAC (std_ss++bmr_ss) [bir_updateB_desc_var_def,
+      bir_updateB_desc_OK_def, bir_updateB_desc_value_def,
+      bir_updateB_desc_exp_def, bmr_ok_def, type_of_bir_val_def,
+      bir_machine_lifted_mem_OK_def, bmr_mem_var_def,
+      bir_is_lifted_exp_def, bir_is_lifted_mem_exp_def] >>
+    CONJ_TAC >- METIS_TAC[size_of_bir_immtype_INJ] >>
+    Cases_on `use_temp` >> (
+      METIS_TAC[EVERY_MEM, bmr_vars_DECLARED, bmr_temp_vars_DECLARED,
+        bmr_vars_IN_TEMP, bir_temp_var_REWRS]
+    )
+  )
+) >>
+`ALL_DISTINCT (MAP (\up. bir_var_name (bir_updateB_desc_var up)) updates)` by (
+  `ALL_DISTINCT (MAP (\up. bir_var_name (bir_updateB_desc_var up)) (updates_imm ++ updates_mem))`
+     suffices_by (METIS_TAC[sortingTheory.ALL_DISTINCT_PERM,sortingTheory.PERM_MAP]) >>
+
+  SIMP_TAC list_ss [ALL_DISTINCT_APPEND] >>
+  Tactical.REVERSE CONJ_TAC >- (
+    Cases_on `mem_up` >> REV_FULL_SIMP_TAC list_ss [] >>
+    FULL_SIMP_TAC (list_ss++bmr_ss) [MEM_MAP, bmr_mem_var_def] >>
+    METIS_TAC[]
+  ) >>
+
+  Q.ABBREV_TAC `imm_up_vars = (MAP (\x. ((case (FST x) of BMLI v v2 => v), SND x)) imm_ups)` >>
+
+  `ALL_DISTINCT (MAP (bir_var_name o FST) imm_up_vars)` by (
+
+    `ALL_DISTINCT (MAP bir_var_name (MAP (\i. case i of BMLI v v2 => v) r.bmr_imms))` by (
+      Q.PAT_X_ASSUM `bmr_ok r` MP_TAC >>
+      SIMP_TAC list_ss [bmr_ok_def,  bmr_varnames_distinct_def, MAP_APPEND,
+        bmr_vars_def, ALL_DISTINCT_APPEND]
+    ) >>
+
+    `(MAP (\i. case i of BMLI v v2 => v) r.bmr_imms) = (MAP FST imm_up_vars)` by (
+      Q.UNABBREV_TAC `imm_up_vars` >>
+      `r.bmr_imms = MAP FST imm_ups` by
+         FULL_SIMP_TAC std_ss [bir_is_lifted_inst_block_COMPUTE_imm_ups_COND_NO_UPDATES_def] >>
+       ASM_SIMP_TAC std_ss [MAP_MAP_o, combinTheory.o_DEF]
+    ) >>
+    FULL_SIMP_TAC std_ss [] >>
+    FULL_SIMP_TAC std_ss [MAP_MAP_o]
+  ) >>
+
+  `(MAP (\up. bir_var_name (bir_updateB_desc_var up)) updates_imm) =
+   (MAP (bir_var_name o FST) (FILTER (IS_SOME o SND) imm_up_vars))` suffices_by
+     METIS_TAC[ALL_DISTINCT_MAP_FILTER] >>
+
+
+   `MAP (\up. bir_var_name (bir_updateB_desc_var up)) updates_imm =
+    MAP (bir_var_name o FST) (MAP (\up. (bir_updateB_desc_var up,bir_updateB_desc_value up))
+        updates_imm)` by (
+      SIMP_TAC std_ss [MAP_MAP_o, combinTheory.o_DEF]
+   ) >>
+   ASM_REWRITE_TAC[] >>
+   Q.UNABBREV_TAC `imm_up_vars` >>
+   ASM_SIMP_TAC std_ss [FILTER_MAP, combinTheory.o_DEF, MAP_MAP_o, pairTheory.pair_CASE_def] >>
+   SIMP_TAC (std_ss++QI_ss++bmr_ss++DatatypeSimps.expand_type_quants_ss[``:'a bir_machine_lifted_imm_t``]) [listTheory.MAP_EQ_f, MEM_FILTER]
+) >>
+
+ASM_SIMP_TAC std_ss [] >>
+
+Cases_on `r.bmr_pc` >> rename1 `BMLPC v_pc v_pc_cond lf_pc` >>
+REPEAT CONJ_TAC >- (
+  METIS_TAC[]
+) >- (
+  Cases_on `eup_temp` >> SIMP_TAC std_ss [bir_updateE_desc_remove_var_REWRS] >>
+  FULL_SIMP_TAC std_ss [] >>
+  REPEAT STRIP_TAC >>
+  `(v' <> mem_v) /\ (!b. v' <> bir_temp_var b mem_v) /\
+   ~(MEM v' (MAP (\i. case i of BMLI v v2 => v) r.bmr_imms)) /\
+   (!b. ~(MEM v' (MAP (\i. case i of BMLI v v2 => bir_temp_var b v) r.bmr_imms)))` by (
+    `v IN {v_pc; v_pc_cond}` by (
+     FULL_SIMP_TAC (std_ss++bmr_ss) [bir_is_lifted_inst_block_COMPUTE_eup_COND_FIXED_VARS_def,
+       IN_INSERT]
+    ) >>
+    Q.PAT_X_ASSUM `brm_ok r` MP_TAC >>
+    ASM_SIMP_TAC (list_ss++bmr_ss++DatatypeSimps.expand_type_quants_ss [``:'a bir_machine_lifted_imm_t``]) [
+      bmr_ok_def, bmr_varnames_distinct_def,
+      bmr_vars_def, bmr_temp_vars_def, bir_temp_var_REWRS, MAP_MAP_o,
+      ALL_DISTINCT_APPEND, MEM_MAP, combinTheory.o_DEF, PULL_EXISTS,
+      FORALL_BOOL] >>
+    FULL_SIMP_TAC std_ss [IN_INSERT, NOT_IN_EMPTY] >>
+       METIS_TAC [bir_temp_var_REWRS]
+  ) >>
+
+  Cases_on `v' IN bir_vars_of_exp (bir_updateB_desc_exp up)` >- METIS_TAC[] >>
+  Cases_on `up` >> rename1 `BUpdateDescB v_up e_up val_up tmp_up` >>
+  FULL_SIMP_TAC (list_ss++bmr_ss++DatatypeSimps.expand_type_quants_ss [``:'a bir_machine_lifted_imm_t``]) [MEM_MAP, bir_updateB_desc_exp_def] >- (
+     `?lf. MEM (BMLI v_up lf) r.bmr_imms` by METIS_TAC[bir_updateB_desc_var_def] >>
+     FULL_SIMP_TAC std_ss [bir_vars_of_updateB_desc_def, IN_INSERT,
+       bir_updateB_desc_temp_var_def] >> (
+       METIS_TAC[]
+     )
+  ) >>
+  Cases_on `mem_up` >> REV_FULL_SIMP_TAC list_ss [] >>
+  REV_FULL_SIMP_TAC list_ss [] >>
+  REPEAT BasicProvers.VAR_EQ_TAC >>
+  FULL_SIMP_TAC (std_ss++bmr_ss) [bir_updateB_desc_var_def, bmr_mem_var_def] >>
+  REPEAT BasicProvers.VAR_EQ_TAC >>
+  FULL_SIMP_TAC std_ss [bir_vars_of_updateB_desc_def, IN_INSERT,
+       bir_updateB_desc_temp_var_def, bir_updateB_desc_var_def] >> (
+       METIS_TAC[]
+  )
+) >- (
+  Cases_on `eup_temp` >> SIMP_TAC std_ss [bir_updateE_desc_remove_var_REWRS] >>
+  METIS_TAC[]
+));
+
+
+
+val bir_is_lifted_inst_block_COMPUTE_OPTIMISED = store_thm (
+"bir_is_lifted_inst_block_COMPUTE_OPTIMISED",
 ``!r. bmr_ok r ==> !mu. WI_wfe mu ==> !mm l.
   ((WF_bmr_ms_mem_contains mm) /\ WI_is_sub (bmr_ms_mem_contains_interval mm) mu) ==>
   !ms_case_cond bl l'.
@@ -565,22 +947,18 @@ val bir_is_lifted_inst_block_COMPUTE_SPLIT = store_thm ("bir_is_lifted_inst_bloc
            bmr_ms_mem_contains r ms mm ==>
            (BL_Address (bmr_pc_lf r ms) = l) ==>
 
-     ?ms' al_step imm_ups mem_up al_mem eup updates. (
+     ?ms' al_step imm_ups mem_up al_mem eup eup_temp updates. (
 
      bir_is_lifted_inst_block_COMPUTE_ms'_COND_WITH_DESC_OK r bs ms al_step ms' /\
      bir_is_lifted_inst_block_COMPUTE_imm_ups_COND_NO_UPDATES r ms ms' imm_ups /\
      bir_is_lifted_inst_block_COMPUTE_mem_COND_NO_UPDATES r ms ms' mem_up /\
      bir_is_lifted_inst_block_COMPUTE_al_mem_COND_WITH_DESC_OK r mu bs ms ms' al_mem /\
-     bir_is_lifted_inst_block_COMPUTE_eup_COND_FIXED_VARS r eup ms' /\
-
-     (* Everything fits with respect to temps etc. *)
-     bir_is_lifted_inst_block_COMPUTE_mem_COND_UPDATES r bs ms ms' mem_up updates /\
-     bir_is_lifted_inst_block_COMPUTE_imm_ups_COND_UPDATES r ms ms' imm_ups updates /\
-     bir_update_block_desc_OK bs.bst_environ eup updates /\
+     bir_is_lifted_inst_block_COMPUTE_eup_COND_FIXED_VARS r bs eup ms' /\
+     bir_is_lifted_inst_block_COMPUTE_updates_FULL r bs mem_up imm_ups eup eup_temp updates /\
 
      (* The block does not depend on the actual values for the state, but just
         the expressions. So, bl should be independent of the actual state. *)
-     (bl = (bir_update_assert_block l' (al_mem++al_step) eup updates)))) ==>
+     (bl = (bir_update_assert_block l' (al_mem++al_step) (if eup_temp then eup else bir_updateE_desc_remove_var eup) updates)))) ==>
   bir_is_lifted_inst_block (r: ('a, 'b, 'ms) bir_lifting_machine_rec_t) ms_case_cond l mu mm (bl :'o bir_block_t)
 ``,
 
@@ -591,15 +969,22 @@ FULL_SIMP_TAC std_ss [bir_is_lifted_inst_block_COMPUTE_imm_ups_COND_THM,
   bir_is_lifted_inst_block_COMPUTE_mem_COND_THM, EVERY_APPEND,
   bir_is_lifted_inst_block_COMPUTE_ms'_COND_WITH_DESC_OK_def,
   bir_is_lifted_inst_block_COMPUTE_al_mem_COND_WITH_DESC_OK_def] >>
-METIS_TAC[bir_is_lifted_inst_block_COMPUTE_eup_COND_FIXED_VARS_THM]);
+METIS_TAC[bir_is_lifted_inst_block_COMPUTE_eup_COND_FIXED_VARS_THM,
+          bir_is_lifted_inst_block_COMPUTE_updates_FULL_THM,
+          bir_is_lifted_inst_block_COMPUTE_eup_COND_remove_var]);
 
 
 
+(*------------------------------------------------------------------*)
+(* Lemmata to help using bir_is_lifted_inst_block_COMPUTE_OPTIMISED *)
+(*------------------------------------------------------------------*)
 
+(* To instantiate bir_is_lifted_inst_block_COMPUTE_OPTIMISED various
+   lemmata and even more auxiliary definitions are handy. These are developed below. *)
 
-(************************)
+(* .....................*)
 (* Deriving assert_desc *)
-(************************)
+(* .....................*)
 
 val bir_assert_desc_OK_via_lifting = store_thm ("bir_assert_desc_OK_via_lifting",
 ``!env e b.
@@ -610,20 +995,412 @@ SIMP_TAC std_ss [bir_is_lifted_exp_def, bir_is_lifted_imm_exp_def,
   bir_assert_desc_OK_def]);
 
 
+(* .................................. *)
+(* efficient checking of imm_ups_COND *)
+(* .................................. *)
 
-(*******************)
-(* Weaken EUP cond *)
-(*******************)
+val bir_is_lifted_inst_block_COMPUTE_imm_ups_COND_NO_UPDATES_CHECK_def = Define `
+  (bir_is_lifted_inst_block_COMPUTE_imm_ups_COND_NO_UPDATES_CHECK ms ms' [] [] <=> T) /\
+  (bir_is_lifted_inst_block_COMPUTE_imm_ups_COND_NO_UPDATES_CHECK ms ms'
+     ((BMLI v lf, NONE)::imm_ups) ((BMLI v' lf')::imms) <=>
+       (v' = v) /\ (lf' = lf) /\
+       (lf ms' = lf ms) /\
+       bir_is_lifted_inst_block_COMPUTE_imm_ups_COND_NO_UPDATES_CHECK ms ms' imm_ups imms
+     ) /\
+  (bir_is_lifted_inst_block_COMPUTE_imm_ups_COND_NO_UPDATES_CHECK ms ms'
+     ((BMLI v lf, SOME res)::imm_ups) ((BMLI v' lf')::imms) <=>
+       (v' = v) /\ (lf' = lf) /\
+       (lf ms' = res) /\
+       bir_is_lifted_inst_block_COMPUTE_imm_ups_COND_NO_UPDATES_CHECK ms ms' imm_ups imms
+     ) /\
+  (bir_is_lifted_inst_block_COMPUTE_imm_ups_COND_NO_UPDATES_CHECK ms ms'
+     _ _ <=> F)`
+
+
+val bir_is_lifted_inst_block_COMPUTE_imm_ups_COND_NO_UPDATES_EVAL = store_thm (
+  "bir_is_lifted_inst_block_COMPUTE_imm_ups_COND_NO_UPDATES_EVAL",
+``!r ms ms' imm_ups.
+  bir_is_lifted_inst_block_COMPUTE_imm_ups_COND_NO_UPDATES r ms ms' imm_ups <=>
+  bir_is_lifted_inst_block_COMPUTE_imm_ups_COND_NO_UPDATES_CHECK ms ms' imm_ups r.bmr_imms``,
+
+SIMP_TAC std_ss [bir_is_lifted_inst_block_COMPUTE_imm_ups_COND_NO_UPDATES_def,
+  bir_is_lifted_inst_block_COMPUTE_imm_ups_COND_NO_UPDATES_CHECK_def] >>
+REPEAT STRIP_TAC >>
+CONV_TAC SYM_CONV >>
+Q.ABBREV_TAC `bmr_imms = r.bmr_imms` >>
+Q.ID_SPEC_TAC `bmr_imms` >> UNABBREV_ALL_TAC >>
+
+Induct_on `imm_ups` >- (
+  Cases_on `bmr_imms` >> SIMP_TAC list_ss [bir_is_lifted_inst_block_COMPUTE_imm_ups_COND_NO_UPDATES_CHECK_def]
+) >>
+Cases >> rename1 `(qq, res_opt)` >>
+Cases_on `qq` >> rename1 `BMLI v lf` >>
+
+Cases >- SIMP_TAC list_ss [bir_is_lifted_inst_block_COMPUTE_imm_ups_COND_NO_UPDATES_CHECK_def] >>
+rename1 `_ _ (XX::bmr_imms')` >>
+Cases_on `XX` >>
+SIMP_TAC (list_ss++bmr_ss) [DISJ_IMP_THM, FORALL_AND_THM] >>
+Cases_on `res_opt` >> (
+  ASM_SIMP_TAC (list_ss++boolSimps.EQUIV_EXTRACT_ss) [bir_is_lifted_inst_block_COMPUTE_imm_ups_COND_NO_UPDATES_CHECK_def]
+));
+
+
+
+(* .............................. *)
+(* efficient checking of mem_COND *)
+(* .............................. *)
+
+val bir_is_lifted_inst_block_COMPUTE_mem_COND_NO_UPDATES_EVAL = store_thm (
+  "bir_is_lifted_inst_block_COMPUTE_mem_COND_NO_UPDATES_EVAL",
+
+``(!r ms ms'. bir_is_lifted_inst_block_COMPUTE_mem_COND_NO_UPDATES r ms ms' NONE <=>
+     (bmr_mem_lf r ms' = bmr_mem_lf r ms)) /\
+
+  (!r ms ms' res. bir_is_lifted_inst_block_COMPUTE_mem_COND_NO_UPDATES r ms ms' (SOME res) <=>
+     (bmr_mem_lf r ms' = res))``,
+
+SIMP_TAC std_ss [bir_is_lifted_inst_block_COMPUTE_mem_COND_NO_UPDATES_def,
+  pairTheory.pair_case_thm, bmr_mem_lf_def] >>
+REPEAT STRIP_TAC >> (
+  Cases_on ` r.bmr_mem` >>
+  SIMP_TAC (std_ss++bmr_ss) []
+));
+
+val bir_is_lifted_inst_block_COMPUTE_al_mem_COND_WITH_DESC_OK_INTRO_NONE = store_thm (
+  "bir_is_lifted_inst_block_COMPUTE_al_mem_COND_WITH_DESC_OK_INTRO_NONE",
+``!r mu bs ms ms'.
+   bir_is_lifted_inst_block_COMPUTE_mem_COND_NO_UPDATES r ms ms' NONE ==>
+   bir_is_lifted_inst_block_COMPUTE_al_mem_COND_WITH_DESC_OK
+            r mu bs ms ms' []``,
+
+SIMP_TAC list_ss [bir_is_lifted_inst_block_COMPUTE_al_mem_COND_WITH_DESC_OK_def,
+  bir_is_lifted_inst_block_COMPUTE_al_mem_COND_def,
+  bir_is_lifted_inst_block_COMPUTE_mem_COND_NO_UPDATES_def,
+  pairTheory.pair_case_thm, bmr_mem_lf_def] >>
+REPEAT STRIP_TAC >>
+Q.EXISTS_TAC `[]` >>
+Cases_on `r.bmr_mem` >>
+FULL_SIMP_TAC (list_ss++bmr_ss) []);
+
+
+(* ......................... *)
+(* efficient checking of eup *)
+(* ......................... *)
 
 val bir_is_lifted_inst_block_COMPUTE_eup_COND_FIXED_VARS_REMOVE_VAR = store_thm (
  "bir_is_lifted_inst_block_COMPUTE_eup_COND_FIXED_VARS_REMOVE_VAR",
 
-``!r eup ms'. bir_is_lifted_inst_block_COMPUTE_eup_COND_FIXED_VARS r eup ms' ==>
-bir_is_lifted_inst_block_COMPUTE_eup_COND_FIXED_VARS r (bir_updateE_desc_remove_var eup) ms'``,
+``!r bs eup ms'. bir_is_lifted_inst_block_COMPUTE_eup_COND_FIXED_VARS r bs eup ms' ==>
+bir_is_lifted_inst_block_COMPUTE_eup_COND_FIXED_VARS r bs (bir_updateE_desc_remove_var eup) ms'``,
 
 SIMP_TAC std_ss [bir_is_lifted_inst_block_COMPUTE_eup_COND_FIXED_VARS_def,
-  bir_updateE_desc_remove_var_REWRS]);
+  bir_updateE_desc_remove_var_REWRS, bir_updateE_desc_OK_remove_var]);
 
+
+
+val bir_is_lifted_inst_block_COMPUTE_eup_COND_FIXED_VARS___JMP =
+store_thm ("bir_is_lifted_inst_block_COMPUTE_eup_COND_FIXED_VARS___JMP",
+``!r bs ms'. bir_is_lifted_inst_block_COMPUTE_eup_COND_FIXED_VARS r bs (BUpdateDescE_Jmp (BL_Address (bmr_pc_lf r ms'))) ms'``,
+
+SIMP_TAC std_ss [bir_is_lifted_inst_block_COMPUTE_eup_COND_FIXED_VARS_def,
+  bir_updateE_desc_var_def, bir_updateE_SEM_def,
+  bir_updateE_desc_OK_def, bir_updateE_desc_exp_def]);
+
+
+val bir_is_lifted_inst_block_COMPUTE_eup_COND_FIXED_VARS___CJMP =
+store_thm ("bir_is_lifted_inst_block_COMPUTE_eup_COND_FIXED_VARS___CJMP",
+``!r bs ms ms'.
+   bmr_ok r ==>
+   bmr_rel r bs ms ==>
+   !c l_t l_f.
+   (bmr_pc_lf r ms' = (if c then l_t else l_f)) ==>
+   !e_c.
+   (bir_is_lifted_exp bs.bst_environ e_c (BLV_Imm (bool2b c))) ==>
+
+   bir_is_lifted_inst_block_COMPUTE_eup_COND_FIXED_VARS r bs
+     (BUpdateDescE_CJmp
+        (SOME (bmr_pc_var_cond r))
+        e_c c (BL_Address l_t) (BL_Address l_f)) ms'``,
+
+REPEAT GEN_TAC >>
+Cases_on `r.bmr_pc` >> rename1 `BMLPC pc_v pc_cond_v lf` >>
+ASM_SIMP_TAC (std_ss++bmr_ss) [bir_is_lifted_inst_block_COMPUTE_eup_COND_FIXED_VARS_def,
+  bir_updateE_desc_var_def, bir_updateE_SEM_def,
+  bir_updateE_desc_OK_def, bir_updateE_desc_exp_def,
+  bir_updateE_desc_value_def, bmr_ok_def, bmr_pc_lf_def,
+  bir_machine_lifted_pc_OK_def, type_of_bool2b,
+  BType_Bool_def, bmr_pc_var_cond_def,
+  bir_is_lifted_exp_def, bir_is_lifted_imm_exp_def
+] >>
+REPEAT STRIP_TAC >- (
+  `EVERY (bir_env_var_is_declared bs.bst_environ) (bmr_temp_vars r)` by
+     METIS_TAC[bmr_temp_vars_DECLARED] >>
+  `MEM pc_cond_v (bmr_temp_vars r)` by (
+     ASM_SIMP_TAC (list_ss++bmr_ss) [bmr_temp_vars_def]
+  ) >>
+  METIS_TAC[EVERY_MEM]
+) >>
+METIS_TAC[]);
+
+
+val bir_is_lifted_inst_block_COMPUTE_eup_COND_FIXED_VARS___XJMP =
+store_thm ("bir_is_lifted_inst_block_COMPUTE_eup_COND_FIXED_VARS___XJMP",
+``!r bs ms ms'.
+   bmr_ok r ==>
+   bmr_rel r bs ms ==>
+   !e.
+   (bir_is_lifted_exp bs.bst_environ e (BLV_Imm (bmr_pc_lf r ms'))) ==>
+
+   bir_is_lifted_inst_block_COMPUTE_eup_COND_FIXED_VARS r bs
+     (BUpdateDescE_XJmp
+        (SOME (bmr_pc_var r))
+        e (bmr_pc_lf r ms')) ms'``,
+
+REPEAT GEN_TAC >>
+Cases_on `r.bmr_pc` >> rename1 `BMLPC pc_v pc_cond_v lf` >>
+ASM_SIMP_TAC (std_ss++bmr_ss) [bir_is_lifted_inst_block_COMPUTE_eup_COND_FIXED_VARS_def,
+  bir_updateE_desc_var_def, bir_updateE_SEM_def,
+  bir_updateE_desc_OK_def, bir_updateE_desc_exp_def,
+  bir_updateE_desc_value_def, bmr_ok_def, bmr_pc_lf_def,
+  bir_machine_lifted_pc_OK_def, type_of_bool2b,
+  BType_Bool_def, bmr_pc_var_def,
+  bir_is_lifted_exp_def, bir_is_lifted_imm_exp_def
+] >>
+REPEAT STRIP_TAC >>
+`EVERY (bir_env_var_is_declared bs.bst_environ) (bmr_temp_vars r)` by
+   METIS_TAC[bmr_temp_vars_DECLARED] >>
+`MEM pc_v (bmr_temp_vars r)` by (
+   ASM_SIMP_TAC (list_ss++bmr_ss) [bmr_temp_vars_def]
+) >>
+METIS_TAC[EVERY_MEM]);
+
+
+
+(* ..................................................................... *)
+(* efficiently checking of bir_is_lifted_inst_block_COMPUTE_updates_FULL *)
+(* ..................................................................... *)
+
+
+
+val bir_is_lifted_inst_block_COMPUTE_updates_FULL_REL_def = Define
+  `bir_is_lifted_inst_block_COMPUTE_updates_FULL_REL
+      (r: ('a, 'b, 'c) bir_lifting_machine_rec_t) bs
+      (mem_up : ('a word -> 'b word) option)
+      (imm_ups :('c bir_machine_lifted_imm_t # bir_imm_t option) list)
+      all_var_names updates_imm update_mem_opt <=>
+
+     (* imm_ups covered *)
+     ((MAP (\up. (bir_updateB_desc_var up, bir_updateB_desc_value up)) updates_imm) =
+      (MAP (\x. (case x of | (BMLI v _, SOME r) => (v, BVal_Imm r)))
+        (FILTER (\x. IS_SOME (SND x)) imm_ups))) /\
+
+     (* mem_up covered *)
+     (case mem_up of NONE => (update_mem_opt = NONE) | SOME res =>
+       (?upd_mem. (update_mem_opt = SOME upd_mem) /\
+           (bir_updateB_desc_var upd_mem = bmr_mem_var r) /\
+           (bir_updateB_desc_value upd_mem =
+             (bir_eval_exp (bir_updateB_desc_exp upd_mem) bs.bst_environ)) /\
+           (bir_is_lifted_exp bs.bst_environ (bir_updateB_desc_exp upd_mem)
+             (BLV_Mem res)))) /\
+
+     (* imm_ups are lifted properly *)
+     (!var e v use_temp.
+            MEM (BUpdateDescB var e (BVal_Imm v) use_temp) updates_imm ==>
+            bir_is_lifted_imm_exp bs.bst_environ e v) /\
+
+     (* Vars fit *)
+     let updates = updates_imm ++ (option_CASE update_mem_opt [] (\x. [x])) in (
+
+     (!i j var.
+        i < LENGTH updates /\ j < i /\
+        var IN bir_vars_of_exp (bir_updateB_desc_exp (EL i updates)) ==>
+        bir_var_name var <>
+        bir_var_name (bir_updateB_desc_temp_var (EL j updates)))) /\
+
+     (!up var. MEM up updates ==>
+               var IN bir_vars_of_exp (bir_updateB_desc_exp up) ==>
+               (bir_var_name var IN all_var_names))
+`;
+
+
+val bir_is_lifted_inst_block_COMPUTE_updates_FULL_INTRO_raw = prove (
+``!r bs mem_up imm_ups all_var_names updates_imm update_mem_opt eup eup_temp.
+
+      (bir_is_lifted_inst_block_COMPUTE_updates_FULL_REL r bs mem_up imm_ups all_var_names updates_imm update_mem_opt /\
+
+      (!v up v'.
+        eup_temp ==>
+        (bir_updateE_desc_var eup = SOME v) ==>
+        ~(bir_var_name v IN all_var_names)) /\
+     (!v e up v'.
+        (~eup_temp \/ (bir_updateE_desc_var eup = NONE)) ==>
+        (bir_updateE_desc_exp eup = SOME e) ==>
+        v IN bir_vars_of_exp e ==>
+        MEM up (updates_imm ++ (option_CASE update_mem_opt [] (\x. [x]))) ==>
+        v' IN {bir_updateB_desc_temp_var up; bir_updateB_desc_var up} ==>
+        bir_var_name v <> bir_var_name v')) ==>
+
+bir_is_lifted_inst_block_COMPUTE_updates_FULL
+  r bs mem_up imm_ups eup eup_temp (updates_imm ++ (option_CASE update_mem_opt [] (\x. [x])))``,
+
+
+SIMP_TAC std_ss [bir_is_lifted_inst_block_COMPUTE_updates_FULL_def,
+  bir_is_lifted_inst_block_COMPUTE_updates_FULL_REL_def, LET_THM] >>
+REPEAT STRIP_TAC >>
+Q.EXISTS_TAC `updates_imm` >>
+Q.EXISTS_TAC `case update_mem_opt of NONE => [] | SOME x => [x]` >>
+Q.ABBREV_TAC `updates = (updates_imm ++ case update_mem_opt of NONE => [] | SOME x => [x])` >>
+ASM_SIMP_TAC std_ss [sortingTheory.PERM_REFL] >>
+REPEAT STRIP_TAC >- (
+  Cases_on `mem_up` >> FULL_SIMP_TAC list_ss []
+) >> (
+  METIS_TAC[]
+));
+
+
+val bir_is_lifted_inst_block_COMPUTE_updates_UPDATES_VARS_def =
+  Define `bir_is_lifted_inst_block_COMPUTE_updates_UPDATES_VARS updates =
+    BIGUNION (IMAGE (\up. {bir_var_name (bir_updateB_desc_temp_var up); bir_var_name (bir_updateB_desc_var up)}) (set updates))`;
+
+
+
+val bir_is_lifted_inst_block_COMPUTE_updates_FULL_INTRO = store_thm (
+"bir_is_lifted_inst_block_COMPUTE_updates_FULL_INTRO",
+``!r bs mem_up imm_ups all_var_names updates_imm update_mem_opt eup eup_temp.
+
+bir_is_lifted_inst_block_COMPUTE_updates_FULL_REL r bs mem_up imm_ups all_var_names updates_imm update_mem_opt ==>
+
+     ((!v up v'.
+        eup_temp ==>
+        (bir_updateE_desc_var eup = SOME v) ==>
+        ~(bir_var_name v IN all_var_names)) /\
+     (!v e up v'.
+        (~eup_temp \/ (bir_updateE_desc_var eup = NONE)) ==>
+        (bir_updateE_desc_exp eup = SOME e) ==>
+        v IN bir_vars_of_exp e ==>
+        ~(bir_var_name v IN (bir_is_lifted_inst_block_COMPUTE_updates_UPDATES_VARS
+           (updates_imm ++ (option_CASE update_mem_opt [] (\x. [x]))))))) ==>
+
+bir_is_lifted_inst_block_COMPUTE_updates_FULL
+  r bs mem_up imm_ups eup eup_temp (updates_imm ++ (option_CASE update_mem_opt [] (\x. [x])))``,
+
+REPEAT STRIP_TAC >>
+MATCH_MP_TAC bir_is_lifted_inst_block_COMPUTE_updates_FULL_INTRO_raw >>
+Q.EXISTS_TAC `all_var_names` >>
+FULL_SIMP_TAC std_ss [
+  bir_is_lifted_inst_block_COMPUTE_updates_UPDATES_VARS_def,
+  IN_BIGUNION, IN_IMAGE,
+  GSYM RIGHT_FORALL_OR_THM, IN_INSERT,
+  NOT_IN_EMPTY] >>
+METIS_TAC[]);
+
+
+
+val bir_is_lifted_inst_block_COMPUTE_updates_UPDATES_VARS_REWRS =
+store_thm ("bir_is_lifted_inst_block_COMPUTE_updates_UPDATES_VARS_REWRS",
+ ``(bir_is_lifted_inst_block_COMPUTE_updates_UPDATES_VARS [] = {}) /\
+   (!e v vn ty ups. (bir_is_lifted_inst_block_COMPUTE_updates_UPDATES_VARS
+      ((BUpdateDescB (BVar vn ty) e v T)::ups) =
+      ((bir_temp_var_name vn) INSERT vn INSERT
+      (bir_is_lifted_inst_block_COMPUTE_updates_UPDATES_VARS ups)))) /\
+
+   (!e v vn ty ups. (bir_is_lifted_inst_block_COMPUTE_updates_UPDATES_VARS
+      ((BUpdateDescB (BVar vn ty) e v F)::ups) =
+      (vn INSERT
+       (bir_is_lifted_inst_block_COMPUTE_updates_UPDATES_VARS ups))))``,
+
+SIMP_TAC list_ss [bir_is_lifted_inst_block_COMPUTE_updates_UPDATES_VARS_def,
+  IMAGE_EMPTY, BIGUNION_EMPTY, IMAGE_INSERT,
+  bir_updateB_desc_temp_var_def, bir_temp_var_REWRS,
+  bir_updateB_desc_var_def, INSERT_INSERT, BIGUNION_INSERT,
+  INSERT_UNION_EQ, UNION_EMPTY, bir_var_name_def]);
+
+
+val bir_is_lifted_inst_block_COMPUTE_updates_FULL_REL___INTRO_NO_MEM =
+store_thm ("bir_is_lifted_inst_block_COMPUTE_updates_FULL_REL___INTRO_NO_MEM",
+``!r bs. bir_is_lifted_inst_block_COMPUTE_updates_FULL_REL r bs NONE [] {} [] NONE``,
+SIMP_TAC list_ss [bir_is_lifted_inst_block_COMPUTE_updates_FULL_REL_def,
+  LET_THM]);
+
+
+val bir_is_lifted_inst_block_COMPUTE_updates_FULL_REL___INTRO_MEM =
+store_thm ("bir_is_lifted_inst_block_COMPUTE_updates_FULL_REL___INTRO_MEM",
+``!r bs e mres.
+   bir_is_lifted_exp bs.bst_environ e (BLV_Mem mres) ==>
+   bir_is_lifted_inst_block_COMPUTE_updates_FULL_REL r bs (SOME mres) [] (IMAGE bir_var_name (bir_vars_of_exp e)) []
+       (SOME (BUpdateDescB (bmr_mem_var r) e (bir_eval_exp e bs.bst_environ) F))``,
+
+SIMP_TAC list_ss [bir_is_lifted_inst_block_COMPUTE_updates_FULL_REL_def,
+  LET_THM, bir_updateB_desc_exp_def, bir_updateB_desc_value_def,
+  bir_updateB_desc_var_def, IN_IMAGE] >>
+REPEAT STRIP_TAC >- (
+  `i = 0` by DECIDE_TAC >>
+  FULL_SIMP_TAC std_ss []
+) >- (
+  METIS_TAC[]
+));
+
+
+val bir_is_lifted_inst_block_COMPUTE_updates_FULL_REL___ADD_IMM_UP_NONE =
+store_thm ("bir_is_lifted_inst_block_COMPUTE_updates_FULL_REL___ADD_IMM_UP_NONE",
+``!r bs mem_up imm_ups all_var_names updates_imm update_mem_opt var lf.
+
+   bir_is_lifted_inst_block_COMPUTE_updates_FULL_REL r bs mem_up imm_ups all_var_names updates_imm update_mem_opt ==>
+
+   bir_is_lifted_inst_block_COMPUTE_updates_FULL_REL r bs mem_up
+       ((BMLI var lf, NONE)::imm_ups) all_var_names updates_imm update_mem_opt``,
+
+SIMP_TAC (list_ss++bmr_ss) [bir_is_lifted_inst_block_COMPUTE_updates_FULL_REL_def,
+  bir_updateB_desc_var_def, bir_updateB_desc_value_def, pairTheory.pair_case_thm, LET_THM] >>
+METIS_TAC[]);
+
+
+
+
+val bir_is_lifted_inst_block_COMPUTE_updates_FULL_REL___ADD_IMM_UP =
+store_thm ("bir_is_lifted_inst_block_COMPUTE_updates_FULL_REL___ADD_IMM_UP",
+``!r bs mem_up imm_ups all_var_names updates_imm update_mem_opt.
+
+   bir_is_lifted_inst_block_COMPUTE_updates_FULL_REL r bs mem_up imm_ups all_var_names updates_imm update_mem_opt ==>
+
+   !var lf v e temp.
+   bir_is_lifted_imm_exp bs.bst_environ e v ==>
+   ~(bir_var_name (bir_temp_var temp var) IN all_var_names) ==>
+   bir_is_lifted_inst_block_COMPUTE_updates_FULL_REL r bs mem_up
+       ((BMLI var lf, SOME v)::imm_ups) (IMAGE bir_var_name (bir_vars_of_exp e) UNION all_var_names) ((BUpdateDescB var e (BVal_Imm v) temp)::updates_imm) update_mem_opt``,
+
+REPEAT GEN_TAC >>
+SIMP_TAC std_ss [bir_is_lifted_inst_block_COMPUTE_updates_FULL_REL_def, LET_THM, APPEND,
+  LENGTH] >>
+Q.ABBREV_TAC `updates =  (updates_imm ++
+            case update_mem_opt of NONE => [] | SOME x => [x])` >>
+
+SIMP_TAC (list_ss++bmr_ss) [bir_is_lifted_inst_block_COMPUTE_updates_FULL_REL_def,
+  bir_updateB_desc_var_def, bir_updateB_desc_value_def, pairTheory.pair_case_thm, LET_THM,
+  bir_updateB_desc_t_11, bir_val_t_11, bir_updateB_desc_exp_def, bir_updateB_desc_value_def] >>
+REPEAT STRIP_TAC >> REPEAT (BasicProvers.VAR_EQ_TAC) >| [
+  METIS_TAC[],
+  METIS_TAC[],
+
+  Cases_on `i` >- (
+    FULL_SIMP_TAC std_ss []
+  ) >>
+  rename1 `j < SUC i'` >>
+  FULL_SIMP_TAC list_ss [arithmeticTheory.ADD_CLAUSES] >>
+  Q.ABBREV_TAC `up = (EL i' updates)` >>
+  `MEM up updates` by METIS_TAC[MEM_EL] >>
+  Cases_on `j` >- (
+    FULL_SIMP_TAC list_ss [bir_updateB_desc_temp_var_def] >>
+    METIS_TAC[]
+  ) >>
+  FULL_SIMP_TAC list_ss [] >>
+  METIS_TAC[],
+
+  FULL_SIMP_TAC std_ss [bir_updateB_desc_exp_def, IN_IMAGE] >>
+  METIS_TAC[],
+
+  METIS_TAC[]
+]);
 
 
 val _ = export_theory();
